%%%%%%%%%%%%%%%%%%%%%%%%%%%%%%%%%%%%%%%%%
% Author: Sibi <sibi@psibi.in>
%%%%%%%%%%%%%%%%%%%%%%%%%%%%%%%%%%%%%%%%%
\documentclass{article}
\usepackage{graphicx}
\usepackage{verbatim}
\usepackage{amsmath}
\usepackage{amsfonts}
\usepackage{amssymb}
\usepackage{tabularx}
\usepackage{mathtools}
\newcommand{\BigO}[1]{\ensuremath{\operatorname{O}\bigl(#1\bigr)}}
\setlength\parskip{\baselineskip}
\begin{document}
\title{Chapter 5 (Section 5.3)}
\author{Sibi}
\date{\today}
\maketitle

% See here: http://tex.stackexchange.com/a/43009/69223
\DeclarePairedDelimiter\abs{\lvert}{\rvert}%
\DeclarePairedDelimiter\norm{\lVert}{\rVert}%

% Swap the definition of \abs* and \norm*, so that \abs
% and \norm resizes the size of the brackets, and the 
% starred version does not.
\makeatletter
\let\oldabs\abs
\def\abs{\@ifstar{\oldabs}{\oldabs*}}
%
\let\oldnorm\norm
\def\norm{\@ifstar{\oldnorm}{\oldnorm*}}
\makeatother
\newpage

\section{Solution 1}
$R^{-1}(p) = $ the person immediately right to $p.$

\section{Solution 2}
$F^{-1}(X) = \text{unique } Y \text{ such that} F(Y) = X$.
So, \begin{align*}
      F(Y) = X \\
      A \setminus Y = X \\
      A \setminus X = Y \\ \\
      F^{-1}(X) = A \setminus X
    \end{align*}

\section{Solution 3}
We will try to find a function $g: R \to R$ such that $f \circ g =
i_\mathbb{R}$ and $g \circ f = i_\mathbb{R}$.

We are hoping to find $g = f^{-1}$. So, $f(x) = \text{unique }y$ such
that $f^{-1}(y) = x$. So, $\frac{2x + 5}{3} = y$. Solving it, we get
$x = \frac{3y-5}{2}$. So, $g(x) = \frac{3x-5}{2}$.

Let's check for $f \circ g = id$.
\begin{align*}
  f(g(x)) \\
  = f(\frac{3x-5}{2}) \\
  = \frac{3x - 5 + 5}{3} \\
  = x \\
  = id_{\mathbb{R}}(x)
\end{align*}

Let's check for $g \circ f = id $
\begin{align*}
  g(f(x)) \\
  = g(\frac{2x + 5}{3}) \\
  = \frac{2x + 5 - 5}{2} \\
  = x \\
  = id_{\mathbb{R}}(x)
\end{align*}

From theorem 5.3.4, we can conclude that $f$ is one-to-one and onto.

\section{Solution 4}
We will try to find a function $g: R \to R$ such that $f \circ g =
i_\mathbb{R}$ and $g \circ f = i_\mathbb{R}$.

We are hoping to find $g = f^{-1}$. So, $f(x) = \text{unique }y$ such
that $f^{-1}(y) = x$. So, $2x^3 - 3 = y$. Solving it, we get
$x = (\frac{3+y}{2})^{1/3}$. So, $g(x) = (\frac{3+x}{2})^{1/3}$.

Let's check for $f \circ g = id$.
\begin{align*}
  f \circ g(x) \\
  = f((\frac{3+x}{2})^{1/3}) \\
  = 3 + x - 3 \\
  = x \\
  = id_R \\
\end{align*}

Similarly, $g \circ f = id_R$

From theorem 5.3.4, we can conclude that $f$ is one-to-one and onto.

\section{Solution 5}
We will try to find a function $g: R^{+} \to R$ such that $f \circ g =
i_\mathbb{R^{+}}$ and $g \circ f = i_\mathbb{R}$.

We are hoping to find $g = f^{-1}$. So, $f(x) = \text{unique }y$ such
that $f^{-1}(y) = x$.So,
\begin{align*}
  10^{2-x} = y \\
  \log_{10}10^{2-x} = \log_{10}y \\
  2 - x = log_{10}y \\
  x = 2 - log y
\end{align*}

So, $g(x) = 2 - log(x)$. Let's verify $f \circ g = id_{\mathbb{R^{+}}}$

\begin{align*}
  f \circ g(x) \\
  = f(2 - log x) \\
  = 10^{2 + log x - 2} \\
  = 10^{log x} \\
  = x \\
  = id_{\mathbb{R^{+}}}
\end{align*}

Also, let's check $g \circ f = id_R$
\begin{align*}
  g \circ f(x) \\
  = g(10^{2 - x}) \\
  = 2 - log_{10} 10^{2-x}\\
  = 2 - (2 - x) \\
  = x \\
\end{align*}

From theorem 5.3.4, we can conclude that $f$ is one-to-one and onto.
\end{document}
